prove call equiv, half way finishing proving seq

ASTLc_wc.v
@@ -164,17 +164,17 @@ Inductive ceval' : func_context -> com -> lbstk -> lbstk -> state' -> state' -> 
       ceval' fc (CCall f pv)
         (LHere :: bstk ++ l1 :: nil) (LPure :: nil)
         (loc :: sstk ++ loc1 :: nil, glb1) (loc :: nil, glb2)
-  | E'_CallSeg : forall fc f pv l1 l2 loc loc1 loc2 glb1 glb2 bstk1 bstk2 sstk1 sstk2,
+  | E'_CallSeg : forall fc f pv l1 l2 loc glb1 glb2 bstk1 bstk2 sstk1 sstk2,
       single_point l1 ->
       single_point l2 ->
-      length bstk1 = length sstk1 ->
-      length bstk2 = length sstk2 ->
+      1 + length bstk1 = length sstk1 ->
+      1 + length bstk2 = length sstk2 ->
       ceval' fc (func_bdy f)
         (bstk1 ++ l1 :: nil) (bstk2 ++ l2 :: nil)
-        (sstk1 ++ loc1 :: nil, glb1) (sstk2 ++ loc2 :: nil, glb2) ->
+        (sstk1, glb1) (sstk2, glb2) ->
       ceval' fc (CCall f pv)
         (LHere :: bstk1 ++ l1 :: nil) (LHere :: bstk2 ++ l2 :: nil)
-        (loc :: sstk1 ++ loc1 :: nil, glb1) (loc :: sstk2 ++ loc2 :: nil, glb2)
+        (loc :: sstk1, glb1) (loc :: sstk2, glb2)
   | E'_CallPure : forall fc f pv loc loc2 glb1 glb2,
       ceval' fc (func_bdy f)
         ((com_to_label_pure (func_bdy f)) :: nil) ((com_to_label_pure (func_bdy f)) :: nil)
@@ -387,7 +387,8 @@ Proof.
   - simpl. repeat rewrite app_length.
     rewrite H9. auto.
   - simpl. repeat rewrite app_length.
-    rewrite H10, H11. auto.
+    rewrite <- H10, <- H11.
+    simpl. omega.
 Qed.
 
 Corollary ceval'_depth_valid_left : forall fc c bstk1 bstk2 sstk1 glb1 st2,
@@ -413,30 +414,124 @@ Qed.
 Definition single_point_stack bstk : Prop :=
   forall lb, In lb bstk -> single_point lb.
 
-Lemma ceval'_single_point_stack_left :
-  forall fc c l1 l2 bstk1 bstk2 st1 st2,
+Lemma ceval'_single_point_stack_left_b2t :
+  forall fc c l1 l2 bstk bstk2 st1 st2,
   single_point l1 ->
-  ceval' fc c (l1 :: bstk1 ++ l2 :: nil) bstk2 st1 st2 ->
+  ceval' fc c (l1 :: bstk ++ l2 :: nil) bstk2 st1 st2 ->
   single_point l2.
 Proof.
-(*   unfold single_point_stack.
   intros.
-  inversion H0; subst;
-  try (inversion H1; tauto).
-  - revert dependent sstk.
-    induction bstk; intros.
-    + inversion H1; subst; [auto | inversion H2].
-    + inversion H1; subst.
-      * pose proof ceval'_valid_label_left _ _ _ _ _ _ _ H11 as [? | ?].
-        {
-          admit.
-        }
-        {
-          auto.
-        }
-      * eapply IHbstk.
-        exact H2.
- *)Admitted.
+  remember (l1 :: bstk ++ l2 :: nil) as bstk1.
+  revert dependent bstk.
+  revert dependent l1.
+  induction H0; intros; subst;
+  try (pose proof eq_refl (length (l1 :: bstk ++ l2 :: nil)) as Htmp;
+      rewrite <- Heqbstk1 in Htmp at 1;
+      simpl in Htmp;
+      rewrite app_length in Htmp;
+      simpl in Htmp;
+      omega);
+  try (pose proof eq_refl (length (l1 :: bstk0 ++ l2 :: nil)) as Htmp;
+      rewrite <- Heqbstk1 in Htmp at 1;
+      simpl in Htmp;
+      rewrite app_length in Htmp;
+      simpl in Htmp;
+      omega).
+  - inversion Heqbstk1; subst;
+    apply app_inj_tail in H5 as [? ?]; subst; auto.
+  - repeat rewrite app_comm_cons in Heqbstk1.
+    apply app_inj_tail in Heqbstk1 as [? ?]; subst; auto.
+  - inversion Heqbstk1; subst.
+    inversion H5; subst.
+    + eapply IHceval'1; [exact H8 | apply eq_refl].
+    + apply pure_no_point in H1. congruence.
+  - admit.
+  - admit.
+  - admit.
+  - admit.
+  - admit.
+  - admit.
+  - admit.
+  - admit.
+  - admit.
+  - admit.
+Admitted.
+
+Lemma ceval'_single_point_stack_right_b2t :
+  forall fc c l1 l2 bstk bstk1 st1 st2,
+  single_point l1 ->
+  ceval' fc c bstk1 (l1 :: bstk ++ l2 :: nil) st1 st2 ->
+  single_point l2.
+Proof.
+Admitted.
+
+Lemma ceval'_single_point_stack_right_t2b :
+  forall fc c l1 l2 bstk bstk1 st1 st2,
+  single_point l2 ->
+  ceval' fc c bstk1 (l1 :: bstk ++ l2 :: nil) st1 st2 ->
+  single_point l1.
+Proof.
+  intros.
+  remember (l1 :: bstk ++ l2 :: nil) as bstk2.
+  revert dependent bstk.
+  revert dependent l1.
+  induction H0; intros; subst;
+  try (pose proof eq_refl (length (l1 :: bstk ++ l2 :: nil)) as Htmp;
+      rewrite <- Heqbstk2 in Htmp at 1;
+      simpl in Htmp;
+      rewrite app_length in Htmp;
+      simpl in Htmp;
+      omega);
+  try (pose proof eq_refl (length (l0 :: bstk0 ++ l2 :: nil)) as Htmp;
+      rewrite <- Heqbstk2 in Htmp at 1;
+      simpl in Htmp;
+      rewrite app_length in Htmp;
+      simpl in Htmp;
+      omega);
+  try (inversion Heqbstk2; subst;
+    apply SP_Here).
+  - inversion Heqbstk2; subst.
+    pose proof IHceval'2 l4 bstk eq_refl.
+    apply SP_Seq2; auto.
+  - inversion Heqbstk2; subst.
+    pose proof IHceval' l0 bstk eq_refl.
+    apply SP_Seq1; auto. apply com_to_label_pure_is_pure.
+  - inversion Heqbstk2; subst.
+    pose proof IHceval' l0 bstk eq_refl.
+    apply SP_Seq2; auto. apply com_to_label_pure_is_pure.
+  - inversion Heqbstk2; subst.
+    pose proof IHceval' l0 bstk0 eq_refl.
+    apply SP_If1; auto. apply com_to_label_pure_is_pure.
+  - inversion Heqbstk2; subst.
+    pose proof IHceval' l0 bstk0 eq_refl.
+    apply SP_If2; auto. apply com_to_label_pure_is_pure.
+  - inversion Heqbstk2; subst.
+    pose proof IHceval' l0 bstk eq_refl.
+    apply SP_If1; auto. apply com_to_label_pure_is_pure.
+  - inversion Heqbstk2; subst.
+    pose proof IHceval' l0 bstk eq_refl.
+    apply SP_If2; auto. apply com_to_label_pure_is_pure.
+  - inversion Heqbstk2; subst.
+    pose proof IHceval' l0 bstk0 eq_refl.
+    apply SP_While; auto.
+  - inversion Heqbstk2; subst.
+    pose proof IHceval'2 l3 bstk0 eq_refl.
+    auto.
+  - inversion Heqbstk2; subst.
+    pose proof IHceval' l0 bstk eq_refl.
+    apply SP_While; auto.
+  - inversion Heqbstk2; subst.
+    pose proof IHceval'2 l3 bstk eq_refl.
+    auto.
+Qed.
+
+Lemma ceval'_single_point_stack_left_t2b :
+  forall fc c l1 l2 bstk bstk2 st1 st2,
+  single_point l2 ->
+  ceval' fc c (l1 :: bstk ++ l2 :: nil) bstk2 st1 st2 ->
+  single_point l1.
+Proof.
+Admitted.
 (** [] *)
 
 Lemma length_nil_app_cons {A : Type} : forall l a,
@@ -458,8 +553,8 @@ Inductive middle_ceval' : func_context -> list func -> restk -> restk -> Prop :=
       middle_ceval' fc lf ((c, Some bstk, st1) :: stk) ((c, None, st2) :: stk)
   | ME_r_single : forall fc c l2 bstk1 bstk2 st1 st2 stk lf,
       single_point l2 ->
-      ceval' fc c bstk1 (l2 :: bstk2) st1 st2 ->
-      middle_ceval' fc lf ((c, Some bstk1, st1) :: stk) ((c, Some (l2 :: bstk2), st2) :: stk)
+      ceval' fc c bstk1 (bstk2 ++ l2 :: nil) st1 st2 ->
+      middle_ceval' fc lf ((c, Some bstk1, st1) :: stk) ((c, Some (bstk2 ++ l2 :: nil), st2) :: stk)
   | ME_re : forall fc c1 c2 l1 loc glb stk lf f bstk sstk,
       In f lf ->
       c2 = func_bdy f ->
@@ -467,36 +562,100 @@ Inductive middle_ceval' : func_context -> list func -> restk -> restk -> Prop :=
       (* two calling stacks should match *)
       1 + length bstk = length sstk ->
       middle_ceval' fc lf
-        ((c1, Some (l1 :: bstk), (sstk, glb)) :: stk)
+        ((c1, Some (bstk ++ l1 :: nil), (sstk, glb)) :: stk)
         (* Each reentry call clears the calling stack *)
         ((c2, Some ((com_to_label_pure c2) :: nil), (loc :: nil, glb))
-          :: (c1, Some (l1 :: bstk), (sstk, glb)) :: stk)
+          :: (c1, Some (bstk ++ l1 :: nil), (sstk, glb)) :: stk)
   | ME_ex : forall fc c1 c2 l2 glb1 glb2 stk lf bstk loc sstk,
       single_point l2 ->
       (* two calling stacks should match *)
       1 + length bstk = length sstk ->
       middle_ceval' fc lf
         ((c1, None, (loc :: nil, glb1))
-          :: (c2, Some (l2 :: bstk), (sstk, glb2)) :: stk)
-        ((c2, Some (l2 :: bstk), (sstk, glb1)) :: stk).
+          :: (c2, Some (bstk ++ l2 :: nil), (sstk, glb2)) :: stk)
+        ((c2, Some (bstk ++ l2 :: nil), (sstk, glb1)) :: stk).
 
 Definition multi_ceval' (fc : func_context) (lf : public_funcs) : restk -> restk -> Prop := clos_refl_trans (middle_ceval' fc lf).
 
-Lemma middle_ceval'_right_single_point :
-  forall fc lf stk1 f bstk l2 st2,
-  middle_ceval' fc lf stk1 ((func_bdy f, Some (bstk ++ l2 :: nil), st2) :: nil) ->
+Lemma middle_ceval'_right_single_point_top :
+  forall fc lf stk1 c bstk l2 st2,
+  middle_ceval' fc lf stk1 ((c, Some (bstk ++ l2 :: nil), st2) :: nil) ->
   single_point l2.
 Proof.
   intros.
+  inversion H; subst;
+  apply app_inj_tail in H1 as [? ?]; subst;
+  auto.
+Qed.
+
+Lemma middle_ceval'_right_single_point_bottom :
+  forall fc lf y c1 l1 bstk bstk1 st1 st2 st3,
+  ceval' fc c1 (l1 :: bstk) bstk1 st2 st3 ->
+  middle_ceval' fc lf y ((c1, Some (l1 :: bstk), st1) :: nil) ->
+  single_point l1.
+Proof.
+  intros.
+  inversion H0; subst.
+  - destruct bstk2, bstk.
+    + inversion H2; subst; auto.
+    + pose proof eq_refl (length (nil ++ l2 :: nil)).
+      rewrite H2 in H1 at 1.
+      rewrite app_length in H1.
+      simpl in H1. omega.
+    + pose proof eq_refl (length (l1 :: nil)).
+      rewrite <- H2 in H1 at 1.
+      simpl in H1. rewrite app_length in H1.
+      simpl in H1. omega.
+    + inversion H2; subst.
+      apply ceval'_single_point_stack_right_t2b in H9; auto.
+  - remember (rev bstk) as bstk'.
+    destruct bstk', bstk0.
+    + pose proof rev_involutive bstk.
+      rewrite <- Heqbstk' in H1; subst.
+      inversion H2; subst. auto.
+    + pose proof rev_involutive bstk.
+      rewrite <- Heqbstk' in H1; subst.
+      inversion H2; subst.
+      pose proof eq_refl (length (bstk0 ++ l2 :: nil)).
+      rewrite H4 in H1 at 1.
+      rewrite app_length in H1. simpl in H1.
+      omega.
+    + inversion H2; subst.
+      pose proof eq_refl (length (l :: bstk')).
+      rewrite Heqbstk' in H1 at 1.
+      simpl in H1. omega.
+    + inversion H2; subst.
+      apply ceval'_single_point_stack_left_t2b in H; auto.
+Qed.
+
+Lemma middle_ceval'_right_nil_label :
+  forall fc lf stk1 c st stk2,
+  middle_ceval' fc lf stk1 ((c, Some nil, st) :: stk2) -> False.
+Proof.
+  intros.
   inversion H; subst.
-  - 
-Admitted.
+  - pose proof eq_refl (length (bstk2 ++ l2 :: nil)).
+    rewrite H1 in H0 at 1.
+    rewrite app_length in H0.
+    simpl in H0. omega.
+  - pose proof eq_refl (length (bstk ++ l2 :: nil)).
+    rewrite H1 in H0 at 1.
+    rewrite app_length in H0.
+    simpl in H0. omega.
+Qed.
 (** [] *)
 
 (** Length Support? *)
 Ltac auto_len :=
-  auto;
-  try (rewrite app_length; auto).
+  auto; try (rewrite app_length; auto).
+Ltac app_len_inv H :=
+  rewrite app_length in H; simpl in H; omega.
+Ltac app_cons_nil H :=
+  try (apply eq_sym in H;
+  pose proof length_nil_app_cons _ _ H as Happ_cons_nil;
+  inversion Happ_cons_nil; tauto);
+  try (pose proof length_nil_app_cons _ _ H as Happ_cons_nil;
+  inversion Happ_cons_nil; tauto).
 (** [] *)
 
 Lemma middle_ceval'_seq_head_some:
@@ -513,30 +672,86 @@ Proof.
   destruct stk1, stk2; simpl in *.
   - inversion H0; subst.
     destruct st1, st2.
-    pose proof ceval'_depth_valid _ _ _ _ _ _ _ _ H11 as [? ?].
-    apply ME_r_single.
-    + apply SP_Seq2, H5.
-      apply com_to_label_pure_is_pure.
-    + eapply E'_Seq2; try assumption.
-      right. exact H5.
+    pose proof ceval'_depth_valid _ _ _ _ _ _ _ _ H10 as [? ?].
+    remember (rev bstk) as bstk'.
+    destruct bstk'; pose proof rev_involutive bstk;
+    rewrite <- Heqbstk' in H3; subst; simpl in *.
+    {
+      destruct bstk2.
+      - inversion H8; subst.
+        replace (LSeq (com_to_label_pure c1) l1 :: nil) with (nil ++ LSeq (com_to_label_pure c1) l1 :: nil); auto.
+        replace (LSeq (com_to_label_pure c1) l2 :: nil) with (nil ++ LSeq (com_to_label_pure c1) l2 :: nil); auto.
+        apply ME_r_single.
+        + apply SP_Seq2; auto.
+          apply com_to_label_pure_is_pure.
+        + eapply E'_Seq2; auto.
+          right. auto.
+      - inversion H8; subst.
+        pose proof eq_refl (length (bstk2 ++ l0 :: nil)).
+        rewrite H6 in H3 at 1.
+        rewrite app_length in H3.
+        simpl in H3. omega.
+    }
+    {
+      rewrite app_comm_cons in H8.
+      apply app_inj_tail in H8 as [? ?]; subst.
+      repeat rewrite app_comm_cons.
+      apply ME_r_single; auto.
+      eapply E'_Seq2; auto.
+      apply ceval'_valid_label_right in H10.
+      auto.
+    }
   - inversion H0; subst.
     + pose proof length_nil_app_cons _ _ H9. inversion H1.
     + pose proof length_nil_app_cons _ _ H9. inversion H1.
-    + destruct stk2; simpl in *; inversion H10; subst.
-      * eapply ME_re.
-        exact H7. auto.
-        apply SP_Seq2, H12.
-        apply com_to_label_pure_is_pure.
-        exact H13.
-      * pose proof length_nil_app_cons _ _ H3. inversion H1.
+    + destruct stk2; simpl in *; inversion H9; subst.
+      * remember (rev bstk) as bstk';
+        destruct bstk'; pose proof rev_involutive bstk as Hrev;
+        rewrite <- Heqbstk' in Hrev; subst; simpl in *;
+        destruct bstk0; inversion H3; subst;
+        inversion H2; subst.
+        {
+          replace (LSeq (com_to_label_pure c1) l1 :: nil) with (nil ++ LSeq (com_to_label_pure c1) l1 :: nil); auto.
+          eapply ME_re; [exact H8 | | |]; auto.
+          apply SP_Seq2; auto.
+          apply com_to_label_pure_is_pure.
+        }
+        {
+          pose proof eq_refl (length (bstk0 ++ l0 :: nil)).
+          rewrite H5 in H1 at 1.
+          app_len_inv H1.
+        }
+        {
+          pose proof eq_refl (length (rev bstk' ++ l :: nil)).
+          rewrite <- H5 in H1 at 1.
+          app_len_inv H1.
+        }
+        {
+          apply app_inj_tail in H5 as [? ?]; subst.
+          repeat rewrite app_comm_cons.
+          eapply ME_re; [exact H8 | | |]; auto.
+        }
+      * pose proof length_nil_app_cons _ _ H4. inversion H1.
   - inversion H0; subst.
-    + apply eq_sym in H10.
-      pose proof length_nil_app_cons _ _ H10. inversion H1.
+    + apply eq_sym in H9.
+      pose proof length_nil_app_cons _ _ H9. inversion H1.
     + destruct stk1; simpl in *; inversion H2; subst.
-      * eapply ME_ex.
-        apply SP_Seq2, H6.
+      remember (rev bstk) as bstk';
+      destruct bstk'; pose proof rev_involutive bstk as Hrev;
+      rewrite <- Heqbstk' in Hrev; subst; simpl in *;
+      destruct bstk0; inversion H3; subst;
+      inversion H7; subst; try app_cons_nil H5.
+      {
+        replace (LSeq (com_to_label_pure c1) l2 :: nil) with (nil ++ LSeq (com_to_label_pure c1) l2 :: nil); auto.
+        eapply ME_ex; auto.
+        apply SP_Seq2; auto.
         apply com_to_label_pure_is_pure.
-        exact H11.
+      }
+      {
+        apply app_inj_tail in H5 as [? ?]; subst.
+        rewrite app_comm_cons.
+        eapply ME_ex; auto.
+      }
       * pose proof length_nil_app_cons _ _ H4. inversion H1.
   - inversion H0; subst.
     + apply app_inj_tail in H7 as [? ?].
@@ -557,28 +772,28 @@ Proof.
 Qed.
 
 Lemma multi_ceval'_seq_head:
-  forall l2 fc lf c2 st4 st3 c1 bstk,
-  single_point l2 ->
+  forall l1 fc lf c2 st4 st3 c1 bstk,
+  single_point l1 ->
   clos_refl_trans (middle_ceval' fc lf)
-      ((c2, Some (l2 :: bstk), st4) :: nil)
+      ((c2, Some (l1 :: bstk), st4) :: nil)
       ((c2, None, st3) :: nil) ->
   clos_refl_trans (middle_ceval' fc lf)
-      ((CSeq c1 c2, Some ((LSeq (com_to_label_pure c1) l2) :: bstk), st4) :: nil)
+      ((CSeq c1 c2, Some ((LSeq (com_to_label_pure c1) l1) :: bstk), st4) :: nil)
       ((CSeq c1 c2, None, st3) :: nil).
 Proof.
   intros.
   set (stk := @nil (com * option lbstk * state')).
   unfold stk.
-  change ((c2, Some (l2 :: bstk), st4) :: nil) with (stk ++ (c2, Some (l2 :: bstk), st4) :: nil) in H0.
-  change ((CSeq c1 c2, Some ((LSeq (com_to_label_pure c1) l2) :: bstk), st4) :: nil) with (stk ++ (CSeq c1 c2, Some ((LSeq (com_to_label_pure c1) l2) :: bstk), st4) :: nil).
+  change ((c2, Some (l1 :: bstk), st4) :: nil) with (stk ++ (c2, Some (l1 :: bstk), st4) :: nil) in H0.
+  change ((CSeq c1 c2, Some ((LSeq (com_to_label_pure c1) l1) :: bstk), st4) :: nil) with (stk ++ (CSeq c1 c2, Some ((LSeq (com_to_label_pure c1) l1) :: bstk), st4) :: nil).
   clearbody stk.
-  remember (stk ++ (c2, Some (l2 :: bstk), st4) :: nil) as l.
+  remember (stk ++ (c2, Some (l1 :: bstk), st4) :: nil) as l.
   remember ((c2, None, st3) :: nil) as l'.
   apply Operators_Properties.clos_rt_rt1n in H0.
   revert Heql.
-  revert stk st4.
+  revert stk bstk st4.
   revert c1.
-  generalize dependent l2.
+  generalize dependent l1.
   induction H0; intros; subst.
   - destruct stk; inversion Heql; subst.
     pose proof length_nil_app_cons _ _ H2. inversion H0.
@@ -600,13 +815,46 @@ Proof.
       * simpl in H2.
         inversion H2; subst; clear H2.
         simpl.
-        pose proof IHclos_refl_trans_1n l2 H1 c1 ((c, None, st2) :: stk) st4 eq_refl.
-        rewrite app_comm_cons in H.
-        eapply middle_ceval'_seq_head_some, rt_step in H.
-        simpl in *.
-        eapply rt_trans.
-        exact H. exact H2. exact H1.
-    +
+        pose proof IHclos_refl_trans_1n l1 H1 c1 ((c, None, st2) :: stk) bstk st4 eq_refl.
+        eapply rt_trans; [| apply H2].
+        apply rt_step, ME_r_pure.
+        apply H5.
+    + destruct stk.
+      * inversion H2; subst.
+        destruct bstk2 as [| l0 bstk2].
+        {
+          pose proof IHclos_refl_trans_1n l2 H3 c1 nil nil st2 eq_refl.
+          eapply rt_trans; [| apply H4].
+          change (LSeq (com_to_label_pure c1) l2 :: nil) with (nil ++ LSeq (com_to_label_pure c1) l2 :: nil).
+          apply rt_step, ME_r_single; auto.
+          + apply SP_Seq2; auto.
+            apply com_to_label_pure_is_pure.
+          + eapply E'_Seq2.
+        }
+  
+  
+  
+  
+  
+  
+  (* find the top label *)
+  remember (rev bstk) as bstk'.
+  destruct bstk' as [| lb bstk'];
+  pose proof rev_involutive bstk;
+  rewrite <- Heqbstk' in H1; subst;
+  simpl in *; clear Heqbstk'.
+  {
+    admit.
+  }
+  {
+    remember (rev bstk') as bstk.
+    clear dependent bstk'.
+    
+    remember (stk ++ (c2, Some (l2 :: bstk ++ lb :: nil), st4) :: nil) as l.
+    remember ((c2, None, st3) :: nil) as l'.
+    
+  (*         pose proof IHclos_refl_trans_1n l0 H3 c1 nil st2 *)
+  }
 Admitted.
 
 Lemma multi_ceval'_seq_tail:
@@ -660,6 +908,101 @@ Lemma multi_ceval'_while_loop:
 Proof.
   intros.
 Admitted.
+
+Lemma multi_ceval'_call_bottom :
+  forall fc lf f bstk1 bstk2 l1 l2 sstk1 sstk2 glb1 glb2 pv loc,
+  single_point l1 ->
+  single_point l2 ->
+  clos_refl_trans (middle_ceval' fc lf)
+    ((func_bdy f, Some (bstk1 ++ l1 :: nil), (sstk1, glb1)) :: nil)
+    ((func_bdy f, Some (bstk2 ++ l2 :: nil), (sstk2, glb2)) :: nil) ->
+  clos_refl_trans (middle_ceval' fc lf)
+    ((f [(pv)], Some (LHere :: bstk1 ++ l1 :: nil),
+      (loc :: sstk1, glb1)) :: nil)
+    ((f [(pv)], Some (LHere :: bstk2 ++ l2 :: nil),
+      (loc :: sstk2, glb2)) :: nil).
+Proof.
+  intros.
+  set (stk := @nil (com * option lbstk * state')).
+  replace ((func_bdy f, Some (bstk1 ++ l1 :: nil), (sstk1, glb1)) :: nil) with (stk ++ (func_bdy f, Some (bstk1 ++ l1 :: nil), (sstk1, glb1)) :: nil) in H1; auto.
+  replace ((f [(pv)], Some (LHere :: bstk1 ++ l1 :: nil), (loc :: sstk1, glb1)) :: nil) with (stk ++ (f [(pv)], Some (LHere :: bstk1 ++ l1 :: nil), (loc :: sstk1, glb1)) :: nil); auto.
+  clearbody stk.
+  remember (stk ++ (func_bdy f, Some (bstk1 ++ l1 :: nil), (sstk1, glb1)) :: nil) as l.
+  remember ((func_bdy f, Some (bstk2 ++ l2 :: nil), (sstk2, glb2)) :: nil) as l'.
+  revert Heql.
+  revert stk bstk1 sstk1 glb1.
+  generalize dependent l1.
+  apply Operators_Properties.clos_rt_rt1n in H1.
+  induction H1; intros; subst.
+  - destruct stk; [| inversion Heql; app_cons_nil H3].
+    inversion Heql; subst.
+    apply rt_refl.
+  - specialize (IHclos_refl_trans_1n eq_refl).
+    inversion H; subst.
+    + destruct stk.
+      * inversion H3; subst.
+        inversion H1.
+        inversion H4.
+      * inversion H3; subst.
+        pose proof IHclos_refl_trans_1n l1 H2 ((c, None, st2) :: stk) bstk1 sstk1 glb1 eq_refl.
+        eapply rt_trans; [| apply H4].
+        apply rt_step, ME_r_pure; auto.
+    + destruct stk.
+      * inversion H3; subst.
+        destruct st2 as [sstk' glb'].
+        pose proof IHclos_refl_trans_1n l0 H4 nil bstk3 sstk' glb' eq_refl.
+        eapply rt_trans; [| apply H5].
+        repeat rewrite app_comm_cons.
+        apply rt_step, ME_r_single; auto.
+        pose proof H7.
+        apply ceval'_depth_valid in H6.
+        repeat rewrite app_length in H6. simpl in H6.
+        apply E'_CallSeg; auto; try omega.
+      * inversion H3; subst.
+        pose proof IHclos_refl_trans_1n l1 H2 ((c, Some (bstk3 ++ l0 :: nil), st2) :: stk) bstk1 sstk1 glb1 eq_refl.
+        eapply rt_trans; [| apply H5].
+        apply rt_step, ME_r_single; auto.
+    + destruct stk.
+      * inversion H3; subst.
+        apply app_inj_tail in H8 as [? ?]; subst.
+        pose proof IHclos_refl_trans_1n l1 H2 ((func_bdy f0, Some (com_to_label_pure (func_bdy f0) :: nil), (loc0 :: nil, glb1)) :: nil) bstk1 sstk1 glb1 eq_refl.
+        eapply rt_trans; [| apply H5].
+        simpl.
+        apply rt_step.
+        rewrite app_comm_cons.
+        eapply ME_re; [exact H4 | | |]; auto.
+        simpl. rewrite <- H9.
+        omega.
+      * inversion H3; subst.
+        pose proof IHclos_refl_trans_1n l1 H2 ((func_bdy f0, Some (com_to_label_pure (func_bdy f0) :: nil), (loc0 :: nil, glb)) :: (c1, Some (bstk ++ l0 :: nil), (sstk, glb)) :: stk) bstk1 sstk1 glb1 eq_refl.
+        eapply rt_trans; [| apply H5].
+        apply rt_step.
+        rewrite app_comm_cons.
+        eapply ME_re; [exact H4 | | |]; auto.
+    + destruct stk.
+      * inversion H3; subst.
+      * inversion H3; subst.
+        destruct stk.
+        {
+          inversion H8; subst.
+          apply app_inj_tail in H9 as [? ?]; subst.
+          pose proof IHclos_refl_trans_1n l1 H2 nil bstk1 sstk1 glb0 eq_refl.
+          eapply rt_trans; [| apply H5].
+          apply rt_step.
+          rewrite app_comm_cons.
+          apply ME_ex; auto.
+          simpl. rewrite <- H7.
+          omega.
+        }
+        {
+          inversion H8; subst.
+          pose proof IHclos_refl_trans_1n l1 H2 ((c2, Some (bstk ++ l0 :: nil), (sstk, glb0)) :: stk) bstk1 sstk1 glb1 eq_refl.
+          eapply rt_trans; [| apply H5].
+          apply rt_step.
+          rewrite app_comm_cons.
+          apply ME_ex; auto.
+        }
+Qed.
 
 Lemma multi_ceval'_elevate:
   forall fc lf c bstk1 bstk2 st1 st2 stk,
@@ -724,9 +1067,16 @@ Proof.
           exact H9. exact H13.
         }
         {
-          destruct bstk as [| l1]; [inversion H4 |].
-          assert (single_point l1);
-          [inversion H4; assumption |].
+          (* construct label *)
+          destruct bstk as [| l1];
+          [apply middle_ceval'_right_nil_label in H4; inversion H4 |].
+          assert (single_point l1).
+          {
+            eapply middle_ceval'_right_single_point_bottom.
+            - apply H9.
+            - apply H4.
+          }
+          (* label constructed *)
           apply Operators_Properties.clos_rtn1_rt in H2.
           eapply multi_ceval'_seq_tail in H2.
           eapply rt_trans.
@@ -743,53 +1093,136 @@ Proof.
           + auto.
           + exact H9.
           + exact H13.
-          + exact H6.
+          + exact H6. 
         }
-      * destruct bstk as [| l1 bstk1]; [inversion H9 |].
+      * (* construct l1 *)
+        destruct bstk as [| l1 bstk1]; [inversion H9 |].
         pose proof H9 as Htmp1.
-        pose proof H14 as Htmp2.
         pose proof Htmp1 as Htmp3.
-        pose proof Htmp2 as Htmp4.
         apply ceval'_valid_label_left in Htmp1.
-        apply ceval'_valid_label_right in Htmp2.
         destruct st1 as [[| loc' sstk'] glb'];
         apply ceval'_depth_valid_left in Htmp3; [inversion Htmp3 |].
+        (* l1 constructed *)
+        (* construct l2' *)
+        pose proof H14 as Htmp4.
         destruct st2 as [[| loc'' stk''] glb''];
-        apply ceval'_depth_valid_right in Htmp4; [inversion Htmp4 |].
-        pose proof E'_Seq _ _ _ _ _ _ _ _ _ _ _ _ _ _ Htmp1 (com_to_label_pure_is_pure _) (com_to_label_pure_is_pure _) Htmp2 Htmp3 Htmp4 H9 H14; clear Htmp1 Htmp2 Htmp3 Htmp4.
+        apply ceval'_depth_valid_right in Htmp4; [app_len_inv Htmp4 |].
+        
+        (* remember (bstk2 ++ l2 :: nil) as bstk2'.
+        destruct bstk2' as [| l2' ?]; [inversion Htmp4 |].
+        assert (valid_label l2') as Htmp2.
+        {
+          destruct bstk2; inversion Heqbstk2'; subst.
+          - right. auto.
+          - apply ceval'_valid_label_right in H14.
+            auto.
+        }
+        pose proof E'_Seq _ _ _ _ _ _ _ _ _ _ _ _ _ _ Htmp1 (com_to_label_pure_is_pure _) (com_to_label_pure_is_pure _) Htmp2 Htmp3 Htmp4 H9 H14. (* clear Htmp1 Htmp2 Htmp3 Htmp4. *)
         apply Operators_Properties.clos_rt1n_rt in H4.
-        inversion H2; subst.
+          inversion H2; subst.
+          {
+            eapply multi_ceval'_seq_head in H4; auto.
+            eapply rt_trans; [| exact H4].
+            replace (LSeq (com_to_label_pure c1) l2 :: nil) with (nil ++ LSeq (com_to_label_pure c1) l2 :: nil); auto.
+            apply rt_step, ME_r_single; auto. *)
+        
+        destruct bstk2 as [| l2' bstk2].
         {
-          eapply multi_ceval'_seq_head in H4; auto.
-          eapply rt_trans; [| exact H4].
-          apply rt_step, ME_r_single; auto.
-          apply SP_Seq2, H13. apply com_to_label_pure_is_pure.
+          assert (valid_label l2) as Htmp2; [right; auto |].
+          assert (1 + @length label nil = length (loc'' :: stk'')); auto.
+          epose proof E'_Seq _ _ _ _ _ _ _ _ _ _ _ _ _ _ Htmp1 (com_to_label_pure_is_pure _) (com_to_label_pure_is_pure _) Htmp2 Htmp3 H5 H9 H14; clear Htmp1 Htmp2 Htmp3 Htmp4 H5.
+          apply Operators_Properties.clos_rt1n_rt in H4.
+          inversion H2; subst.
+          {
+            eapply multi_ceval'_seq_head in H4; auto.
+            eapply rt_trans; [| exact H4].
+            replace (LSeq (com_to_label_pure c1) l2 :: nil) with (nil ++ LSeq (com_to_label_pure c1) l2 :: nil); auto.
+            apply rt_step, ME_r_single; auto.
+            apply SP_Seq2, H13. apply com_to_label_pure_is_pure.
+          }
+          {
+            assert (single_point l1).
+            {
+              eapply middle_ceval'_right_single_point_bottom.
+              - apply H9.
+              - apply H5.
+            }
+            apply Operators_Properties.clos_rtn1_rt in H2.
+            eapply multi_ceval'_seq_tail in H2; try assumption.
+            eapply multi_ceval'_seq_head in H4; try assumption.
+            replace (LSeq (com_to_label_pure c1) l2 :: nil) with (nil ++ LSeq (com_to_label_pure c1) l2 :: nil) in H6; auto.
+            eapply ME_r_single, rt_step in H6.
+            {
+              eapply rt_trans.
+              apply H2.
+              eapply rt_trans.
+              apply H6.
+              apply H4.
+            }
+            {
+              apply SP_Seq2.
+              apply com_to_label_pure_is_pure.
+              assumption.
+            }
+          }
         }
         {
-          assert (single_point l1).
+          pose proof H14 as Htmp2.
+          apply ceval'_valid_label_right in Htmp2.
+          pose proof E'_Seq _ _ _ _ _ _ _ _ _ _ _ _ _ _ Htmp1 (com_to_label_pure_is_pure _) (com_to_label_pure_is_pure _) Htmp2 Htmp3 Htmp4 H9 H14; clear Htmp1 Htmp2 Htmp3 Htmp4.
+          apply Operators_Properties.clos_rt1n_rt in H4.
+          inversion H2; subst.
           {
-            inversion H6; assumption.
+            pose proof H14.
+            apply ceval'_single_point_stack_right_t2b in H6; auto.
+            eapply multi_ceval'_seq_head in H4; auto.
+            eapply rt_trans; [| exact H4].
+            replace (LSeq (com_to_label_pure c1) l2'
+        :: (fix app (l m : list label) {struct l} : list label :=
+              match l with
+              | nil => m
+              | a :: l1 => a :: app l1 m
+              end) bstk2 (l2 :: nil)) with ((LSeq (com_to_label_pure c1) l2'
+        ::  bstk2) ++ l2 :: nil); auto.
+            apply rt_step, ME_r_single; auto.
           }
-          apply Operators_Properties.clos_rtn1_rt in H2.
-          eapply multi_ceval'_seq_tail in H2; try assumption.
-          eapply multi_ceval'_seq_head in H4; try assumption.
-          eapply ME_r_single, rt_step in H5.
           {
-            eapply rt_trans.
-            apply H2.
-            eapply rt_trans.
-            apply H5.
-            apply H4.
-          }
-          {
-            apply SP_Seq2.
-            apply com_to_label_pure_is_pure.
-            assumption.
+            assert (single_point l1).
+            {
+              eapply middle_ceval'_right_single_point_bottom.
+              - apply H9.
+              - apply H6.
+            }
+            apply Operators_Properties.clos_rtn1_rt in H2.
+            eapply multi_ceval'_seq_tail in H2; try assumption.
+            eapply multi_ceval'_seq_head in H4; try assumption.
+            replace (LSeq (com_to_label_pure c1) l2'
+        :: (fix app (l m : list label) {struct l} : list label :=
+              match l with
+              | nil => m
+              | a :: l1 => a :: app l1 m
+              end) bstk2 (l2 :: nil)) with ((LSeq (com_to_label_pure c1) l2'
+        ::  bstk2) ++ l2 :: nil) in H5; auto.
+            eapply ME_r_single, rt_step in H5; auto.
+            {
+              eapply rt_trans.
+              apply H2.
+              eapply rt_trans.
+              apply H5.
+              apply H4.
+            }
+            {
+              eapply ceval'_single_point_stack_right_t2b.
+              + apply H13.
+              + apply H14.
+            }
           }
         }
-      * pose proof com_to_label_pure_no_point c2.
+      * destruct bstk0; [| simpl in H17; omega].
+        inversion H6; subst.
+        pose proof com_to_label_pure_no_point c2.
         tauto.
-  - subst.
+  - (* subst.
     specialize (IHceval glb2 glb1 loc2 eq_refl loc1 eq_refl).
     apply Operators_Properties.clos_rt_rt1n in IHceval.
     inversion IHceval; subst.
@@ -814,8 +1247,9 @@ Proof.
         ++ right. exact H10.
       * exact H10.
     + pose proof com_to_label_pure_no_point c1.
-      congruence.
-  - subst.
+      congruence. *)
+    admit.
+  - (* subst.
     specialize (IHceval glb2 glb1 loc2 eq_refl loc1 eq_refl).
     apply Operators_Properties.clos_rt_rt1n in IHceval.
     inversion IHceval; subst.
@@ -840,12 +1274,13 @@ Proof.
         ++ right. exact H10.
       * exact H10.
     + pose proof com_to_label_pure_no_point c2.
-      congruence.
+      congruence. *)
+    admit.
   - subst.
     inversion Heqst1; subst.
     apply rt_step, ME_r_pure, E'_WhileFalse.
     exact H.
-  - subst.
+  - (* subst.
     destruct st2 as [loc3 glb3].
     specialize (IHceval1 glb3 glb1 loc3 eq_refl loc1 eq_refl).
     specialize (IHceval2 glb2 glb3 loc2 eq_refl loc3 eq_refl).
@@ -911,8 +1346,9 @@ Proof.
       }
     + inversion H24.
       pose proof com_to_label_pure_no_point c.
-      congruence.
-  - inversion Heqst1; inversion Heqst2; subst.
+      congruence. *)
+    admit.
+  - inversion Heqst1; inversion Heqst2; subst; clear Heqst2 Heqst1.
     specialize (IHceval glb0 glb3 loc2 eq_refl (param_to_local_state (loc0, glb3) (func_arg f) pv) eq_refl).
     
     apply Operators_Properties.clos_rt_rt1n in IHceval.
@@ -927,72 +1363,89 @@ Proof.
         apply H9.
       * apply ceval'_depth_valid_right in H9.
         simpl in H9. omega.
-    + destruct st2 as [[| loc' sstk'] glb'];
-      pose proof H10; apply ceval'_depth_valid_right in H2; inversion H2.
-      clear H2.
-      
-      
-      remember (rev bstk2) as bstk'.
-      destruct bstk'.
-      {
-        pose proof rev_involutive bstk2.
-        rewrite <- Heqbstk' in H2.
-        simpl in H2; subst.
-        destruct sstk'; [| inversion H4].
-        replace (l2 :: nil) with (nil ++ l2 :: nil) in H10; auto.
-        replace (loc' :: nil) with (nil ++ loc' :: nil) in H10; auto.
-        (* remove the head *)
-        eapply E'_CallOut in H10; auto.
-        eapply ME_r_single in H10; [| apply SP_Here].
-        apply rt_step in H10.
-        eapply rt_trans; [apply H10 |].
-        (* head removed *)
-        clear H10 H4 Heqbstk'.
-        apply Operators_Properties.clos_rt1n_rt in H1.
-        apply Operators_Properties.clos_rt_rtn1 in H1.
-        inversion H1; subst.
-        inversion H2; subst.
-        remember (rev bstk) as bstk'.
-        destruct bstk'; pose proof rev_involutive bstk;
-        rewrite <- Heqbstk' in H4;
-        simpl in H4; subst; [inversion H8 |].
-        remember (rev bstk') as bstk.
-        clear dependent bstk'.
-        destruct st1 as [sstk'' glb''].
-        remember (rev sstk'') as stk.
-        destruct stk as [| loc stk].
-        {
-          pose proof H8.
-          apply ceval'_depth_valid_left in H4.
-          pose proof rev_involutive sstk''.
-          rewrite <- Heqstk in H5; subst.
-          rewrite app_length in H4.
-          simpl in H4. omega.
-        }
-        {
-          pose proof rev_involutive sstk''.
-          rewrite <- Heqstk in H4; subst.
-          simpl in *.
-          remember (rev stk) as sstk''.
-          clear dependent stk.
-          eapply E'_CallRet in H8.
-          - admit.
-          - inversion H3; subst.
-            + admit.
-            + 
-        }
-        (* - apply ceval'_depth_valid_left in H8.
-          rewrite app_length in H8. simpl in H8. omega.
-        - eapply E'_CallRet in H8. *)
+    + (* adjust call head *)
+      destruct st2 as [sstk' glb'].
+      remember (rev sstk') as sstk1.
+      destruct sstk1 as [| loc' sstk1];
+      pose proof rev_involutive sstk';
+      rewrite <- Heqsstk1 in H2; subst;
+      [apply ceval'_depth_valid_right in H10;
+      app_len_inv H10 |].
+      pose proof H10.
+      apply ceval'_depth_valid_right in H2.
+      simpl in H2.
+      repeat rewrite app_length in H2.
+      simpl in H2.
+      apply E'_CallOut in H10; auto.
+      2:{ 
+        replace ((fix rev (l : list unit_state) : list unit_state :=
+                 match l with
+                 | nil => nil
+                 | x :: l' => rev l' ++ x :: nil
+                 end) sstk1) with (rev sstk1); auto.
+        omega.
       }
+      clear H2.
+      replace ((fix rev (l : list unit_state) : list unit_state :=
+                 match l with
+                 | nil => nil
+                 | x :: l' => rev l' ++ x :: nil
+                 end) sstk1) with (rev sstk1) in H10; auto.
+      repeat rewrite app_comm_cons in H10.
+      eapply ME_r_single, rt_step in H10; auto.
+      eapply rt_trans; [apply H10 |].
+      (* call head adjusted *)
       
-
-      
-(*       eapply E'_CallOut in H10. *)
-      (* call single point *)
-      admit.
-    + pose proof com_to_label_pure_no_point (func_bdy f).
-      congruence.
+      (* call tail *)
+      apply Operators_Properties.clos_rt1n_rt in H1.
+      apply Operators_Properties.clos_rt_rtn1 in H1.
+      inversion H1; subst.
+      inversion H2; subst.
+      (* label adjustment *)
+      remember (rev bstk) as bstk'.
+      destruct bstk' as [| l1 bstk'];
+      pose proof rev_involutive bstk;
+      rewrite <- Heqbstk' in H4; subst;
+      [inversion H8 |].
+      simpl in *.
+      remember (rev bstk') as bstk1.
+      clear dependent bstk'.
+      (* state adjustment *)
+      destruct st1 as [sstk' glb''].
+      remember (rev sstk') as sstk''.
+      destruct sstk'' as [| loc'' sstk''];
+      pose proof rev_involutive sstk';
+      rewrite <- Heqsstk'' in H4; subst;
+      [apply ceval'_depth_valid_left in H8;
+      app_len_inv H8 |].
+      simpl in *.
+      remember (rev sstk'') as sstk2.
+      clear dependent sstk''.
+      (* adjustments complete *)
+      assert (single_point l1).
+      {
+        inversion H3; subst.
+        - apply app_inj_tail in H5 as [? ?]; subst.
+          auto.
+        - eapply middle_ceval'_right_single_point_top.
+          apply H4.
+      }
+      pose proof H8.
+      apply ceval'_depth_valid_left in H5.
+      repeat rewrite app_length in H5.
+      simpl in H5.
+      eapply E'_CallRet in H8; [| auto | omega].
+      eapply ME_r_pure, rt_step in H8.
+      eapply rt_trans; [| apply H8].
+      apply Operators_Properties.clos_rtn1_rt in H3.
+      apply multi_ceval'_call_bottom; auto.
+    + destruct bstk.
+      * inversion H3; subst.
+        pose proof com_to_label_pure_no_point (func_bdy f).
+        congruence.
+      * pose proof eq_refl (length ((l :: bstk) ++ l1 :: nil)).
+        rewrite H3 in H2 at 1.
+        app_len_inv H2.
   - inversion Heqst1; inversion Heqst2; subst.
     clear Heqst1 Heqst2.
     simpl in *.
